\documentclass[a4paper,12pt]{article}

\usepackage[fontset=none]{ctex}
\usepackage{fontspec}
\usepackage{xeCJK}
\usepackage[english]{babel}
\usepackage{hyperref}

\usepackage{amsmath}
\usepackage{amssymb}

\setCJKmainfont[Path="../Assets/Fonts/SourceHan/Serif/",BoldFont={SourceHanSerifSC-Bold.otf},AutoFakeSlant=0.25]{SourceHanSerifSC-Regular.otf}
\setCJKsansfont[Path="../Assets/Fonts/SourceHan/Sans/",BoldFont={SourceHanSansSC-Bold.otf},AutoFakeSlant=0.25]{SourceHanSansSC-Regular.otf}
\setCJKmonofont[Path="../Assets/Fonts/SourceHan/Mono/"]{SourceHanMono.ttc}
\newCJKfontfamily\kaiti[Path="../Assets/Fonts/AR_PL_UKai/"]{ukai.ttc}

\title{Assignment-2}
\author{刘行逸}
\date{20250928}

\hypersetup{
    pdftitle={Assignment-y},
    pdfauthor={刘行逸},
}

\begin{document}
\maketitle

\section*{1}
\addcontentsline{toc}{section}{1}
\begin{table}[h]
    \scriptsize
    \begin{tabular}{cc|cccccc|c}
            &       & $z$ & $x$  & $y$  & $s_1$ & $s_2$ & $s_3$ &      \\
        \hline
            &       & $1$ & $-3$ & $-2$ & $0$   & $0$   & $0$   & $0$  \\
        \hline
            & $s_1$ & $0$ & $2$  & $1$  & $1$   & $0$   & $0$   & $18$ \\
            & $s_2$ & $0$ & $2$  & $3$  & $0$   & $1$   & $0$   & $42$ \\
        $*$ & $s_3$ & $0$ & $3$  & $1$  & $0$   & $0$   & $1$   & $24$ \\
    \end{tabular}
\end{table}

\begin{table}[h]
    \scriptsize
    \begin{tabular}{cc|cccccc|c}
            &       & $z$ & $x$ & $y$                                      & $s_1$ & $s_2$ & $s_3$                                     &                                   \\
        \hline
            &       & $1$ & $0$ & $-2 + 1 = -1$                            & $0$   & $0$   & $0 + 1 = 1$                               & $0 + 24 = 24$                     \\
        \hline
        $*$ & $s_1$ & $0$ & $0$ & $1 - 1 \times \frac{2}{3} = \frac{1}{3}$ & $1$   & $0$   & $0 - 1 \times \frac{2}{3} = -\frac{2}{3}$ & $18 - 24 \times \frac{2}{3} = 2$  \\
            & $s_2$ & $0$ & $0$ & $3 - 1 \times \frac{2}{3} = \frac{7}{3}$ & $0$   & $1$   & $0 - 1 \times \frac{2}{3} = -\frac{2}{3}$ & $42 - 24 \times \frac{2}{3} = 26$ \\
            & $x$   & $0$ & $3$ & $1$                                      & $0$   & $0$   & $1$                                       & $24$                              \\
    \end{tabular}
\end{table}

\begin{table}[h]
    \scriptsize
    \begin{tabular}{cc|cccccc|c}
            &       & $z$ & $x$ & $y$           & $s_1$                 & $s_2$ & $s_3$                                        &                        \\
        \hline
            &       & $1$ & $0$ & $0$           & $0 + 1 \times 3 = 3$  & $0$   & $1 + (-\frac{2}{3} \times 3) = -1$           & $24 + 2 \times 3 = 30$ \\
        \hline
            & $y$   & $0$ & $0$ & $\frac{1}{3}$ & $1$                   & $0$   & $-\frac{2}{3}$                               & $2$                    \\
        $*$ & $s_2$ & $0$ & $0$ & $0$           & $0 - 1 \times 7 = -7$ & $1$   & $-\frac{2}{3} - (-\frac{2}{3}) \times 7 = 4$ & $26 - 2 \times 7 = 12$ \\
            & $x$   & $0$ & $3$ & $0$           & $0 - 1 \times 3 = -3$ & $0$   & $1 - (-\frac{2}{3}) \times 3 = 3$            & $24 - 2 \times 3 = 18$ \\
    \end{tabular}
\end{table}

\begin{table}[h]
    \scriptsize
    \begin{tabular}{cc|cccccc|c}
         &       & $z$ & $x$ & $y$           & $s_1$                                        & $s_2$                                     & $s_3$                          &                                   \\
        \hline
         &       & $1$ & $0$ & $0$           & $3 + (-4) \times \frac{1}{4} = 2$            & $0 + 1 \times \frac{1}{4} = \frac{1}{4}$  & $0$                            & $30 + 12 \times \frac{1}{4} = 33$ \\
        \hline
         & $y$   & $0$ & $0$ & $\frac{1}{3}$ & $1 + (-7) \times \frac{1}{6} = -\frac{1}{6}$ & $0 + 1 \times \frac{1}{6} = \frac{1}{6}$  & $0$                            & $2 + 12 \times \frac{1}{6} = 4$   \\
         & $s_3$ & $0$ & $0$ & $0$           & $-7$                                         & $1$                                       & $4$                            & $12$                              \\
         & $x$   & $0$ & $3$ & $0$           & $-3 - (-7) \times \frac{3}{4} = \frac{9}{4}$ & $0 - 1 \times \frac{3}{4} = -\frac{3}{4}$ & $3 - 4 \times \frac{3}{4} = 0$ & $18 - 12 \times \frac{3}{4} = 9$  \\
    \end{tabular}
\end{table}

\begin{align*}
    \begin{pmatrix}0 & \frac{1}{3} & 0\\0 & 0 &4\\3 & 0 & 0\end{pmatrix} \begin{pmatrix}x\\y\\s_3\end{pmatrix} & = \begin{pmatrix}4\\12\\9\end{pmatrix} \\
    \begin{pmatrix}x\\y\\s_3\end{pmatrix}                                                                      & = \begin{pmatrix}3\\12\\3\end{pmatrix} \\
    \therefore \quad x = 3, \ y = 12,                                                                          & \ \max{(3 x + 2 y)} = 33               \\
\end{align*}

\section*{2}
\addcontentsline{toc}{section}{2}

\section*{3}
\addcontentsline{toc}{section}{3}

\end{document}
