\documentclass[a4paper,12pt]{article}

\usepackage[fontset=none]{ctex}
\usepackage{fontspec}
\usepackage{xeCJK}
\usepackage[english]{babel}

\usepackage{hyperref}

\usepackage{amsmath}
\usepackage{amssymb}
\usepackage{mathtools}

\setCJKmainfont[Path="../Assets/Fonts/SourceHan/Serif/",BoldFont={SourceHanSerifSC-Bold.otf},AutoFakeSlant=0.25]{SourceHanSerifSC-Regular.otf}
\setCJKsansfont[Path="../Assets/Fonts/SourceHan/Sans/",BoldFont={SourceHanSansSC-Bold.otf},AutoFakeSlant=0.25]{SourceHanSansSC-Regular.otf}
\setCJKmonofont[Path="../Assets/Fonts/SourceHan/Mono/"]{SourceHanMono.ttc}
\newCJKfontfamily\kaiti[Path="../Assets/Fonts/AR_PL_UKai/"]{ukai.ttc}

\title{Assignment-5}
\author{刘行逸}
\date{20251125}

\hypersetup{
    pdftitle={Assignment-5},
    pdfauthor={刘行逸},
}

\begin{document}
\maketitle

\section*{1}
\addcontentsline{toc}{section}{1}
\begin{align*}
    f(x)   & = -5 x^2 + 5 x                                 \\
    f^*(y) & = \sup_{x \in \mathbb{R}}{(y x - f(x))}        \\
           & = \sup_{x \in \mathbb{R}}{(y x + 5 x^2 - 5 x)} \\
           & = +\infty, \ (x \to +\infty)                   \\
\end{align*}

Can't plot.

\section*{2}
\addcontentsline{toc}{section}{2}
\begin{align*}
    \because a \le x & \le b , \ f \text{ is convex}                                 \\
    \therefore f(x)  & = f(\frac{b - x}{b - a} a + \frac{x - a}{b - a} b)            \\
                     & = f(\frac{b - x}{b - a} a + (1 - \frac{b - x}{b - a}) b)      \\
                     & \le \frac{b - x}{b - a} f(a) + (1 - \frac{b - x}{b - a}) f(b) \\
                     & = \frac{b - x}{b - a} f(a) + \frac{x - a}{b - a} f(b)         \\
\end{align*}

\section*{3}
\addcontentsline{toc}{section}{3}
\begin{align*}
    \operatorname{dom}{h}                                 & = \operatorname{dom}{f} \cap \operatorname{dom}{g} \\
    \because \operatorname{dom}{f}, \operatorname{dom}{g} & \text{ are convex}                                 \\
    \therefore \operatorname{dom}{h}                      & \text{ is convex}                                  \\
    \forall{(x < y)}                                      & \in \operatorname{dom}{h}, k \in [0, 1]            \\
    h(k x + (1 - k) y)                                    & = f(k x + (1 - k) y) + g(k x + (1 - k) y)          \\
                                                          & \le k f(x) + (1 - k) f(y) + k g(x) + (1 - k) g(y)  \\
                                                          & = k (f(x) + g(x)) + (1 - k) (f(y) + g(y))          \\
                                                          & = k h(x) + (1 - k) h(y)                            \\
    \text{Q.}                                             & \text{E.D.}                                        \\
\end{align*}

\section*{4}
\addcontentsline{toc}{section}{4}
\begin{align*}
    \operatorname{dom}{f}               & = (x,y), \ x, y > 0                                             \\
    \therefore \operatorname{dom}{f}    & \text{ is convex}                                               \\
    (x \log{x})'                        & = \log{x} + 1 > 0, \ x > 0                                      \\
    (x \log{x})''                       & = \frac{1}{x} > 0, \ x > 0                                      \\
    \therefore x \log{x}                & \text{ is convex}                                               \\
    \forall{(x_1, y_1), (x_2, y_2)}     & \in \operatorname{dom}{f}, k \in [0, 1]                         \\
    f(k (x_1, y_1) + (1 - k) (x_2,y_2)) & = f(k x_1 + (1 - k) x_2,k y_1 + (1 - k) y_2)                    \\
                                        & = (k x_1 + (1 - k) x_2) \log{(k x_1 + (1 - k) x_2)}             \\
                                        & \phantom{=} + (k y_1 + (1 - k) y_2) \log{(k y_1 + (1 - k) y_2)} \\
                                        & \le (k x_1 \log{x_1} + (1 - k) x_2 \log{x_2})                   \\
                                        & \phantom{=} + (k y_1 \log{y_1} + (1 - k) y_2 \log{y_2})         \\
                                        & = k (x_1 \log{x_1} + y_1 \log{y_1})                             \\
                                        & \phantom{=} + (1 - k) (x_2 \log{x_2} + y_2 \log{y_2})           \\
                                        & = k f(x_1, y_1) + (1 - k) f(x_2, y_2)                           \\
    \text{Q.}                           & \text{E.D.}                                                     \\
\end{align*}

\section*{5}
\addcontentsline{toc}{section}{5}
\begin{align*}
    {\| y - \theta^T X \|_2}^2           & = (y - \theta^T X)^T (y - \theta^T X)                                                                                                                                           \\
                                         & = y^T y - y^T \theta^T X - X^T \theta y + X^T \theta \theta^T X                                                                                                                 \\
                                         & = (X^T \theta)^2 - 2 y \theta^T X + y^2                                                                                                                                         \\
                                         & = \theta^T (X X^T) \theta - (2 y X^T) \theta + y^2                                                                                                                              \\
    X X^T                                & \in S_{+}^n                                                                                                                                                                     \\
    {\| \theta \|_1}                     & = \sum_{i=1}^{n}{|\theta_i|}                                                                                                                                                    \\
                                         & \ge p^T \theta, \ ((\forall{p}, |p_i| = 1) \land (\exists{p}, p^T \theta = {\| \theta \|_1}))                                                                                   \\
    \therefore {\| \theta \|_1} \le t    & \iff \forall{p, |p_i| = 1}, p^T \theta \le t                                                                                                                                    \\
    Q                                    & = (\prescript{}{1}{p},\prescript{}{2}{p},\prescript{}{3}{p},\cdots,\prescript{}{2^n}{p})^T,                                                                                     \\
    (\forall{i \ne j}                    & \in [1,2^n], (\prescript{}{i}{p} \ne \prescript{}{j}{p}) \land (\forall{k}, |{\prescript{}{i}{p}}_k| = 1))                                                                      \\
    \therefore \text{Lasso regression: } &                                                                                                                                                                                 \\
                                         & \operatorname{Max. }{\frac{1}{2} \theta^T (2 X X^T) \theta + (-2 y X)^T \theta + y^2}                                                                                           \\
    \text{s.t.}                          & \begin{cases}Q \theta \le (t,t,t,\cdots,t)^T, 2 X X^T \in {S_{+}}^n \\ y \in \mathbb{R}, X \in \mathbb{R}^{n+1}, \theta \in \mathbb{R}^{n+1}\end{cases} \\
\end{align*}

\end{document}
